backends/lean/Aeneas/Tactic/Step/Tests/HigherOrder.lean
@@ -1,0 +1,134 @@
+import Aeneas.Std.Slice
+import Aeneas.Tactic.Step
+
+open Aeneas Aeneas.Std Result ControlFlow Error
+
+namespace higher_order
+
+def applyF (f : U32 → Result U32) (x : U32) : Result U32 := f x
+
+@[step]
+theorem applyF_spec (f : U32 → Result U32) (x : U32)
+    (post : U32 → Prop)
+    (hf : f x ⦃ post ⦄) :
+    applyF f x ⦃ post ⦄ := by
+  simp [applyF]; exact hf
+
+/--
+info: Try this:
+
+  [apply]     let* ⟨ y, y_post ⟩ ← [ +inferPost ] applyF_spec
+    case hf => let* ⟨ ⟩ ← [ +inferPost ] U32.add_spec
+    agrind
+-/
+#guard_msgs in
+example (a : U32) (h : a.val + 1 ≤ U32.max) :
+    applyF (fun x => x + 1#u32) a ⦃ y => y.val = a.val + 1 ⦄ := by
+  step*? +inferPost
+
+-- Higher-order in 2 functions, operates on a pair of inputs/outputs
+def callPair (f : U32 → Result U32) (g : U32 → Result U32) (xy : U32 × U32) : Result (U32 × U32) := do
+  let a ← f xy.1
+  let b ← g xy.2
+  return (a, b)
+
+@[step]
+theorem callPair_spec (f g : U32 → Result U32) (xy : U32 × U32)
+    (postF : U32 → Prop) (postG : U32 → Prop)
+    (hf : f xy.1 ⦃ postF ⦄) (hg : g xy.2 ⦃ postG ⦄) :
+    callPair f g xy ⦃ fun p => postF p.1 ∧ postG p.2 ⦄ := by
+  unfold callPair
+  step*
+
+/--
+info: Try this:
+
+  [apply]     let* ⟨ ab, ab_post1, ab_post2 ⟩ ← [ +inferPost ] callPair_spec
+    case hf => let* ⟨ ⟩ ← [ +inferPost ] U32.add_spec
+    case hg => let* ⟨ ⟩ ← [ +inferPost ] U32.add_spec
+    agrind
+-/
+#guard_msgs in
+example (x y : U32) (hx : x.val + 1 ≤ U32.max) (hy : y.val + 2 ≤ U32.max) :
+    callPair (fun a => a + 1#u32) (fun b => b + 2#u32) (x, y) ⦃ ab => ab.1.val = x.val + 1 ∧ ab.2.val = y.val + 2 ⦄ := by
+  step*? +inferPost
+
+-- Calls f then g in sequence
+def callFThenG (f g : U32 → Result U32) (x : U32) : Result U32 := do
+  let y ← f x
+  g y
+
+@[step]
+theorem callFThenG_spec (f g : U32 → Result U32) (x : U32)
+    (mid post : U32 → Prop)
+    (hf : f x ⦃ mid ⦄)
+    (hg : ∀ y, mid y → g y ⦃ post ⦄) :
+    callFThenG f g x ⦃ post ⦄ := by
+  unfold callFThenG
+  step*
+
+/--
+info: Try this:
+
+  [apply]     let* ⟨ y, y_post ⟩ ← [ +inferPost ] callFThenG_spec
+    case hf => let* ⟨ ⟩ ← [ +inferPost ] U32.add_spec
+    case hg =>
+      intros y a✝
+      let* ⟨ ⟩ ← [ +inferPost ] U32.add_spec
+    agrind
+-/
+#guard_msgs in
+example (x : U32) (h1 : x.val + 1 ≤ U32.max) (h2 : x.val + 2 ≤ U32.max) :
+    callFThenG (fun a => a + 1#u32) (fun b => b + 1#u32) x ⦃ y => y.val = x.val + 2 ⦄ := by
+  step*? +inferPost
+
+def callSlicemapM (x : Slice U32) : Result (Slice U32) := do
+  let y ← x.mapM (fun x => x + 1#u32)
+  return y
+
+/--
+info: Try this:
+
+  [apply]     let* ⟨ y, y_post1, y_post2 ⟩ ← [ +inferPost ] Slice.mapM_spec
+    case hf =>
+      intros i hi
+      let* ⟨ ⟩ ← [ +inferPost ] U32.add_spec
+    agrind
+-/
+#guard_msgs in
+example (s : Slice U32) (h : ∀ i (hi : i < s.len), s[i] < U32.max) :
+  callSlicemapM s ⦃ s' =>
+    s'.len = s.len ∧
+    ∀ i (hi₁ : i < s.len) (hi₂ : i < s'.len), s'[i].val = s[i].val + 1
+    ⦄ := by
+  unfold callSlicemapM
+  step*? +inferPost
+
+def callSlicemapMTwice (x : Slice U32) : Result (Slice U32) := do
+  let y ← x.mapM (fun x => x + 1#u32)
+  let z ← y.mapM (fun x => x * x)
+  return z
+
+/--
+info: Try this:
+
+  [apply]     let* ⟨ y, y_post1, y_post2 ⟩ ← [ +inferPost ] Slice.mapM_spec
+    case hf =>
+      intros i hi
+      let* ⟨ ⟩ ← [ +inferPost ] U32.add_spec
+    let* ⟨ z, z_post1, z_post2 ⟩ ← [ +inferPost ] Slice.mapM_spec
+    case hf =>
+      intros i hi
+      let* ⟨ ⟩ ← [ +inferPost ] U32.mul_spec
+    agrind
+-/
+#guard_msgs in
+example (s : Slice U32) (h : ∀ i (hi : i < s.len), (s[i] + 1) * (s[i] + 1) ≤ U32.max) :
+  callSlicemapMTwice s ⦃ s' =>
+    s'.len = s.len ∧
+    ∀ i (hi₁ : i < s.len) (hi₂ : i < s'.len), s'[i].val = (s[i].val + 1) * (s[i].val + 1)
+    ⦄ := by
+  unfold callSlicemapMTwice
+  step*? +inferPost
+
+end higher_order
